Gt3/HasTy/Universe.lean
@@ -1,0 +1,6 @@
+import Gt3.HasTy.Regular
+import Gt3.JEq.Universe
+
+theorem Ctx.HasTy.us (σ : ULevel.Subst) {Γ A a} (h : Ctx.HasTy Γ A a)
+  : Ctx.HasTy (Γ.us σ) (A.us σ) (a.us σ)
+  := (h.refl.us σ).lhs_ty
