Gt3/RwEq/Universe.lean
@@ -1,4 +1,12 @@
 import Gt3.RwEq.Erase
 import Gt3.JEq.Universe
 
---TODO: this
+theorem Ctx.KWEq.us (σ : ULevel.Subst) {Γ a b} (h : Ctx.KWEq Γ a b)
+  : Ctx.KWEq (Γ.us σ) (a.us σ) (b.us σ) := by convert WfEq.us σ h; simp [KWEq]
+
+theorem Ctx.KEq.us (σ : ULevel.Subst) {Γ a b} (h : Ctx.KEq Γ a b)
+  : Ctx.KEq (Γ.us σ) (a.us σ) (b.us σ)
+  := by induction h with
+  | wf_clamp h => exact KEq.wf_clamp (h.us σ)
+  | trans => apply trans <;> assumption
+  | _ => constructor <;> assumption
